Rename MState into archState and Model into archModel
This is done to be consistent with the paper descriptions.

This also remove the MState stack of record that wasn't really useful,
thus removing some boilerplate

Also add improve documentation in TermModels.v

ArchSem/CandidateExecutions.v
@@ -186,7 +186,7 @@ Module CandidateExecutions (IWA : InterfaceWithArch) (Term : TermModelsT IWA) (N
     Record pre {et : exec_type} {nmth : nat} :=
       make_pre {
           (** Initial state *)
-          init : MState.t nmth;
+          init : archState nmth;
           (** Each thread is a list of instruction who each have a trace,
               we force the return type to be unit, but it just means we
               forget the actual value *)
@@ -543,7 +543,7 @@ Module CandidateExecutions (IWA : InterfaceWithArch) (Term : TermModelsT IWA) (N
                   dmap_insert reg val map
                 else map
               ) map itrc.1
-          ) (pe.(init).(MState.regs) !!! tid) (pe.(events) !!! tid).
+          ) (pe.(init).(archState.regs) !!! tid) (pe.(events) !!! tid).
 
       (** Get all the final register map from a pre-execution *)
       Definition final_reg_map pe : vec registerMap nmth :=
@@ -886,7 +886,7 @@ Module CandidateExecutions (IWA : InterfaceWithArch) (Term : TermModelsT IWA) (N
 
       Definition is_valid_init_reg_read pe (eid : EID.t) : iEvent → Prop :=
         is_reg_readP (λ reg _ rv,
-            match pe.(init).(MState.regs) !! eid.(EID.tid) with
+            match pe.(init).(archState.regs) !! eid.(EID.tid) with
             | Some regmap => dmap_lookup reg regmap = Some rv
             | None => False
             end).
@@ -899,7 +899,7 @@ Module CandidateExecutions (IWA : InterfaceWithArch) (Term : TermModelsT IWA) (N
           ∃ reg reg_acc rv,
             (ev = RegRead reg reg_acc &→ rv) ∧
               ∃ H : eid.(EID.tid) < nmth,
-                dmap_lookup reg (pe.(init).(MState.regs) !!! nat_to_fin H) =
+                dmap_lookup reg (pe.(init).(archState.regs) !!! nat_to_fin H) =
                   Some rv.
       Proof.
         unfold is_valid_init_reg_read.
@@ -931,7 +931,7 @@ Module CandidateExecutions (IWA : InterfaceWithArch) (Term : TermModelsT IWA) (N
         addr ← get_addr read;
         val ← get_mem_value read;
         guard' (
-            mem_lookup addr (bvn_n val / 8) pe.(init).(MState.memory)
+            mem_lookup addr (bvn_n val / 8) pe.(init).(archState.memory)
               |$> bv_to_bvn = Some val).
       #[export] Instance is_valid_init_mem_read_dec pe eid :
         Decision (is_valid_init_mem_read pe eid).
@@ -1068,17 +1068,12 @@ Module CandidateExecutions (IWA : InterfaceWithArch) (Term : TermModelsT IWA) (N
 
     Definition final_mem_map (cd : t) : memoryMap :=
       let written_values := final_write_per_addr cd |$> snd in
-      union_with (λ old new, Some new) cd.(init).(MState.memory) written_values.
+      union_with (λ old new, Some new) cd.(init).(archState.memory) written_values.
 
-    Definition cd_to_MState (cd : t) : MState.t nmth :=
-      {|MState.regs := final_reg_map cd;
-        MState.memory := final_mem_map cd;
-        MState.address_space := cd.(init).(MState.address_space)|}.
-
-    Definition cd_to_MState_final (cd : t) (term : terminationCondition nmth) :
-        option (MState.final nmth) :=
-      MState.finalize (MState.MakeI (cd_to_MState cd) term).
-
+    Definition cd_to_archState (cd : t) : archState nmth :=
+      {|archState.regs := final_reg_map cd;
+        archState.memory := final_mem_map cd;
+        archState.address_space := cd.(init).(archState.address_space)|}.
 
     (** ** Memory based relations *)
 
@@ -1245,7 +1240,7 @@ Module CandidateExecutions (IWA : InterfaceWithArch) (Term : TermModelsT IWA) (N
     Definition addr_space_wf cd :=
       ∀ '(eid, ev) ∈ event_list cd,
         if get_addr_space ev is Some a
-        then a = cd.(init).(MState.address_space)
+        then a = cd.(init).(archState.address_space)
         else True.
     Instance addr_space_wf_dec {cd : t} : Decision (addr_space_wf cd).
     Proof. unfold addr_space_wf. tc_solve. Defined.
@@ -1260,14 +1255,14 @@ Module CandidateExecutions (IWA : InterfaceWithArch) (Term : TermModelsT IWA) (N
           ∀ instr ∈ cd.(events) !!! tid,
           ∀ ev ∈ fst instr,
           if get_reg ev is Some reg
-          then reg ∈ dom (cd.(init).(MState.regs) !!! tid)
+          then reg ∈ dom (cd.(init).(archState.regs) !!! tid)
           else True;
         (** All memory operations are in the initial footprint *)
         mem_footprint_valid:
         ∀ '(eid, ev) ∈ event_list cd,
           if get_addr ev is Some addr then
             if get_size ev is Some n then
-              ∀ addr' ∈ addr_range addr n, addr' ∈ dom cd.(init).(MState.memory)
+              ∀ addr' ∈ addr_range addr n, addr' ∈ dom cd.(init).(archState.memory)
             else False
           else True
       }.
@@ -1356,20 +1351,23 @@ Module CandidateExecutions (IWA : InterfaceWithArch) (Term : TermModelsT IWA) (N
 
     Module Res.
       Section Res.
-        Context {et : exec_type}.
-        Context {unspec : Type}.
-        Notation axres := (result string (behavior unspec)).
-        Notation mres := (Model.Res.t unspec).
-        Notation model := (Model.nc unspec).
-        Notation cand := (cand et).
+      Context {et : exec_type}.
+      Context {unspec : Type}.
+      Notation axres := (result string (behavior unspec)).
+      Notation archres := (archModel.res unspec).
+      Notation cand := (cand et).
 
-      Definition to_ModelResult (axr : axres) {n} (cd : cand n)
-        (term : terminationCondition n) : option (mres n) :=
+      Definition to_archModel (axr : axres) {n} (cd : cand n)
+        (term : terminationCondition n) : option (archres n term) :=
         match axr with
-        | Ok Allowed => cd_to_MState_final cd term |$> Model.Res.FinalState
+        | Ok Allowed =>
+            let finalState := cd_to_archState cd in
+            if decide (archState.is_terminated term finalState) is left p then
+              Some (archModel.Res.FinalState finalState p)
+            else None
         | Ok Rejected => None
-        | Ok (Unspecified u) => Some (Model.Res.Unspecified u)
-        | Error msg => Some (Model.Res.Error msg)
+        | Ok (Unspecified u) => Some (archModel.Res.Unspecified u)
+        | Error msg => Some (archModel.Res.Error msg)
         end.
 
       (** When a model gives a more precise definition for the error of another
@@ -1420,10 +1418,10 @@ Module CandidateExecutions (IWA : InterfaceWithArch) (Term : TermModelsT IWA) (N
       Context {et : exec_type}.
       Context {unspec : Type}.
       Notation axres := (result string (behavior unspec)).
-      Notation mres := (Model.Res.t unspec).
-      Notation model := (Model.nc unspec).
+      Notation archres := (archModel.res unspec).
+      Notation model := (archModel.nc unspec).
       Notation t := (t et unspec).
-        Notation cand := (cand et).
+      Notation cand := (cand et).
 
       (** Lifting Res definition to Ax *)
       Definition wider (ax ax' : t) := ∀ n cd, Res.wider (ax n cd) (ax' n cd).
@@ -1454,32 +1452,29 @@ Module CandidateExecutions (IWA : InterfaceWithArch) (Term : TermModelsT IWA) (N
         unfold equiv. intros. apply Res.equiv_is_ok. naive_solver.
       Qed.
 
-      Definition to_ModelResult (ax : t) {n} (cd : cand n)
-        (term : terminationCondition n) : option (mres n) :=
-        Res.to_ModelResult (ax n cd) cd term.
-
-      (** Creates a non-computational model from an instruction semantic and an
-          axiomatic model *)
-      Definition to_Modelnc (isem : iMon ()) (ax : t) : model :=
-        λ n initSt,
-          {[ mr |
+      (** Creates a non-computational architecture model from an instruction
+          semantic and an axiomatic model *)
+      Definition to_archModel_nc (isem : iMon ()) (ax : t) : model :=
+        λ n term initSt,
+          {[ model_result : archres n term |
              ∃ cd : cand n,
                cd.(init) = initSt
                ∧ wf cd
                ∧ ISA_match cd isem
-               ∧ to_ModelResult ax cd initSt.(MState.termCond) = Some mr
+               ∧ Res.to_archModel (ax n cd) cd term = Some model_result
           ]}.
-      #[global] Typeclasses Transparent to_Modelnc.
+      #[global] Typeclasses Transparent to_archModel_nc.
 
       Lemma wider_Model (isem : iMon ()) (ax ax' : t) :
-        wider ax ax' → Model.wider (to_Modelnc isem ax) (to_Modelnc isem ax').
+        wider ax ax' →
+        archModel.wider (to_archModel_nc isem ax) (to_archModel_nc isem ax').
       Proof using.
-        intros WD nmth initSt.
+        intros WD nmth term initSt.
         split.
         all: intros NE.
         all: set_unfold.
         all: repeat split_and.
-        all: intros ?.
+        all: (intros [] ||intros ?).
         all: try split.
         all: intros [cd ?].
         all: specialize (WD nmth cd); unfold Res.wider.
@@ -1487,39 +1482,42 @@ Module CandidateExecutions (IWA : InterfaceWithArch) (Term : TermModelsT IWA) (N
         all: destruct (ax' nmth cd) as [[]|] eqn:Heqn'.
         all: try (eapply NE; clear NE).
         all: (exists cd; intuition).
-        all: unfold to_ModelResult, Res.to_ModelResult in *.
-        all: rewrite Heqn in *.
-        all: rewrite Heqn' in *.
-        all: hauto l:on.
+        all: try rewrite Heqn' in *.
+        all: try rewrite Heqn in *.
+        all: cbn in *.
+        all: try hauto l:on.
         Unshelve.
         all: exact "".
       Qed.
 
       Lemma weaker_Model (isem : iMon ()) (ax ax' : t) :
-        weaker ax ax' → Model.weaker (to_Modelnc isem ax) (to_Modelnc isem ax').
+        weaker ax ax' →
+        archModel.weaker (to_archModel_nc isem ax) (to_archModel_nc isem ax').
       Proof using.
-        intros WD nmth initSt.
+        intros WD nmth term initSt.
         intros NE.
         repeat split_and.
         all: set_unfold.
-        all: intros ? [cd ?].
+        all: (intros [] || intros ?).
+        all: intros [cd ?].
         all: specialize (WD nmth cd); unfold Res.weaker.
         all: destruct (ax nmth cd) as [[]|] eqn:Heqn.
         all: destruct (ax' nmth cd) as [[]|] eqn:Heqn'.
         all: try (eapply NE; clear NE).
         all: (exists cd; intuition).
-        all: unfold to_ModelResult, Res.to_ModelResult in *.
-        all: rewrite Heqn in *.
-        all: rewrite Heqn' in *.
+        all: try rewrite Heqn in *.
+        all: try rewrite Heqn' in *.
+        all: cbn in *.
         all: hauto l:on.
         Unshelve.
         all: exact "".
       Qed.
 
       Lemma equiv_Model (isem : iMon ()) (ax ax' : t) :
-        equiv ax ax' → Model.equiv (to_Modelnc isem ax) (to_Modelnc isem ax').
+        equiv ax ax' →
+        archModel.equiv (to_archModel_nc isem ax) (to_archModel_nc isem ax').
       Proof using.
-        rewrite Model.equiv_weaker.
+        rewrite archModel.equiv_weaker.
         rewrite equiv_weaker.
         intros [].
         split; by apply weaker_Model.
